theories/rule_misc.v
@@ -728,3 +728,4 @@ From HypVeri Require Import RAs.
     destruct r;[contradiction|contradiction|].
     rewrite H1 //.
   Qed.
+
