theories/rules/donate.v
@@ -1,42 +1,64 @@
 From machine_program_logic.program_logic Require Import machine weakestpre.
 From HypVeri Require Import RAs rule_misc lifting rules.rules_base.
 From iris.proofmode Require Import tactics.
-Require Import iris.base_logic.lib.ghost_map.
+From iris.algebra Require Import gset.
 Require Import stdpp.fin.
 
-(* Lemma hvc_mem_donate11 {instr i wi r2 ptx so q sa wf wt} ai r0 r1 j pd : *)
-(*   instr = Hvc -> *)
-(*   decode_instruction wi = Some(instr) -> *)
-(*   decode_hvc_func r0 = Some(Donate) -> *)
-(*   (fin_to_nat r1) ≤ page_size -> *)
-(*   {[pd; (to_pid_aligned ai)]} ⊆ sa -> *)
-(*   pd ∈ so -> *)
-(*   <<i>> ∗ PC @@ i ->r ai ∗ ai ->a wi *)
-(*   ∗ O@i:={q}[so] ∗ A@i:={1}[sa] *)
-(*   ∗ R0 @@ i ->r r0 ∗ R1 @@ i ->r r1 ∗ R2 @@i ->r r2 ∗ TX@ i := ptx *)
-(*   ∗ new_transaction_descriptor11 ptx i wf zero_word wt one_word j pd *)
-(*     ⊢ SSWP ExecI @ i {{ (λ m, ⌜m = HaltI ⌝ ∗ <<i>> ∗ PC @@ i ->r (ai ^+ 1)%f ∗ ai ->a wi *)
-(*   ∗ O@i:={q}[so] ∗ A@i:={1}[sa∖{[pd]}] *)
-(*   ∗ R0 @@ i ->r (encode_hvc_ret_code Succ) ∗ R1 @@ i ->r r1 ∗ TX@ i := ptx *)
-(*   ∗ ∃wh, (R2 @@ i ->r wh ∗ wh ->t{1}(i,wf, wt, {[j := {[pd]}]},Donation) ∗ wh ->re j) *)
-(*   ∗ new_transaction_descriptor11 ptx i zero_word zero_word zero_word one_word j pd)}}%I. *)
-(* Proof. *)
-(*   iIntros (Hinstr Hdecodei Hdecodef Hvalidlen Hsa Hso) "(Htok & HPC & Hai & Hown & Haccess & HR0 & HR1 & HR2 & HTX & Htd)". *)
-(*   iApply (sswp_lift_atomic_step ExecI);[done|]. *)
-(*   iIntros (σ1) "%Hsche Hσ". *)
-(*   inversion Hsche as [ Hcureq ]; clear Hsche. *)
-(*   apply fin_to_nat_inj in Hcureq. *)
-(*   iModIntro. *)
-(*   iDestruct "Hσ" as "(Hcur & Hmem & Hreg & Htxpage & ? & Hownedpt & Haccesspt & Htrans & Hrcv)". *)
-(*   (* valid regs *) *)
-(*   iDestruct ((gen_reg_valid4 σ1 i PC ai R0 r0 R1 r1 R2 r2 Hcureq ) with "Hreg HPC HR0 HR1 HR2 ") *)
-(*     as "[%HPC [%HR0 [%HR1 %HR2]]]";eauto. *)
-(*   (* valid pt *) *)
-(*   iDestruct ((gen_access_valid2 σ1 i 1 sa pd (to_pid_aligned ai)) with "Haccesspt Haccess") as %[Haccpd Haccai];eauto. *)
-(*   (* valid mem *) *)
-(*   iDestruct (gen_mem_valid σ1 ai wi with "Hmem Hai") as %Hmem. *)
-(*   iDestruct (gen_mem_valid_td11 σ1 _ _ _ _ _ _ with "Htd Hmem") as %Htd. *)
-(*   iSplit. *)
-(*   - admit. *)
-(*   - admit. *)
-(*  Admitted. *)
+Section donate.
+
+Context `{vmG: !gen_VMG Σ}.
+
+Lemma hvc_donate {instr i wi r2 pi ptx sown q sacc sexcl q' wf wt des qh sh} {l :Word} {spsd: gset PID}
+      ai r0 r1 j (psd: list PID) :
+  (* the current instruction is hvc *)
+  instr = Hvc ->
+  (* the decoding of wi is correct *)
+  decode_instruction wi = Some(instr) ->
+  (* the instruction is in page pi *)
+  addr_in_page ai pi ->
+  (* the decoding of R0 is FFA_DONATE *)
+  decode_hvc_func r0 = Some(Donate) ->
+  (* l is the number of to-be-donated pages *)
+  (finz.to_z l) = (Z.of_nat (length psd)) ->
+  (* the descriptor, in list Word *)
+  des = serialized_transaction_descriptor i j wf wt l psd W0 ->
+  (* the whole descriptor resides in the TX page *)
+  seq_in_page (of_pid ptx) (length des) ptx ->
+  (* spsd is the gset of all to-be-donated pages *)
+  spsd = (list_to_set psd) ->
+  (* pi and pages in spsd are accessible for VM i *)
+  {[pi]} ∪ spsd ⊆ sacc ->
+  (* VM i owns pages in spsd *)
+  spsd ⊆ sown ->
+  (* pages in spsed are exclusive to VM i *)
+  spsd ⊆ sexcl ->
+  (* there are at least one free handles in the hpool *)
+  sh ≠ ∅ ->
+  {SS{{ ▷(PC @@ i ->r ai) ∗ ▷ ai ->a wi
+  ∗ ▷ O@i:={q}[sown] ∗ ▷ A@i:={1}[sacc] ∗ ▷ E@i:={q'}[sexcl]
+  ∗ ▷ (R0 @@ i ->r r0) ∗ ▷ (R1 @@ i ->r r1) ∗ ▷(R2 @@i ->r r2) ∗  ▷ TX@ i := ptx
+  ∗ ▷ mem_region des ptx
+  ∗ ▷ hp{ qh }[ (GSet sh)] }}}
+   ExecI @ i {{{ RET ExecI ; PC @@ i ->r (ai ^+ 1)%f ∗ ai ->a wi
+  ∗ O@i:={q}[sown] ∗ A@i:={1}[sacc∖spsd] ∗ E@i:={q'}[sexcl]
+  ∗ R0 @@ i ->r (encode_hvc_ret_code Succ) ∗ R1 @@ i ->r r1  ∗ TX@ i := ptx
+  ∗ ∃(wh: Word), ( ⌜ wh ∈ sh ⌝ ∗ R2 @@ i ->r wh ∗ wh ->t{1}(i,wf, wt, {[j := spsd]},Donation)
+  ∗ wh ->re j ∗ R2 @@ i ->r wh ∗ hp{qh}[(GSet (sh∖{[wh]}))] )
+  ∗ mem_region des ptx}}}.
+Proof.
+  Admitted.
+  (* iIntros (Hinstr Hdecodei Hdecodef Hvalidlen Hsa Hso) "(Htok & HPC & Hai & Hown & Haccess & HR0 & HR1 & HR2 & HTX & Htd)". *)
+  (* iApply (sswp_lift_atomic_step ExecI);[done|]. *)
+  (* iIntros (σ1) "%Hsche Hσ". *)
+  (* inversion Hsche as [ Hcureq ]; clear Hsche. *)
+  (* apply fin_to_nat_inj in Hcureq. *)
+  (* iModIntro. *)
+  (* iDestruct "Hσ" as "(Hcur & Hmem & Hreg & Htxpage & ? & Hownedpt & Haccesspt & Htrans & Hrcv)". *)
+  (* (* valid regs *) *)
+  (* iDestruct ((gen_reg_valid4 σ1 i PC ai R0 r0 R1 r1 R2 r2 Hcureq ) with "Hreg HPC HR0 HR1 HR2 ") *)
+  (*   as "[%HPC [%HR0 [%HR1 %HR2]]]";eauto. *)
+  (* (* valid pt *) *)
+  (* iDestruct ((gen_access_valid2 σ1 i 1 sa pd (to_pid_aligned ai)) with "Haccesspt Haccess") as %[Haccpd Haccai];eauto. *)
+  (* (* valid mem *) *)
+  (* iDestruct (gen_mem_valid σ1 ai wi with "Hmem Hai") as %Hmem. *)
+  (* iDestruct (gen_mem_valid_td11 σ1 _ _ _ _ _ _ with "Htd Hmem") as %Htd. *)
